AsyncTest failing

theories/Execute.v
@@ -1,4 +1,7 @@
+From AsyncTest Require Export
+     Operator.
 From FileSync Require Export
+     AsyncTest
      Gen
      Server
      Semantics.
@@ -13,7 +16,9 @@ From Coq Require Export
      ExtrOcamlIntConv
      ExtrOcamlNativeString.
 Import
+  ListNotations
   SumNotations
+  XNotations
   OSys.
 Open Scope sum_scope.
 
@@ -63,57 +68,109 @@ Definition read_file' (p: path) : IO content :=
   close_in_noerr cin;;
   ret (from_ostring ostr).
 
-Definition read_file (p: path) : IO A :=
+Definition read_file (p: path) : IO IR :=
   oc <- catch_any_exc (read_file' p);;
-  ret (if oc is Some c then Aread c else Ano).
+  ret (if oc is Some c then JEncode__String c else JSON__False).
 
-Definition write_file (p: path) (str: content) : IO A :=
+Definition write_file (p: path) (str: content) : IO IR :=
   ou <- catch_any_exc (cout <- open_out (flatten p);;
                    output_string cout str;;
                    close_out_noerr cout);;
-  ret (if ou is Some tt then Ayes else Ano).
+  ret (if ou is Some tt then JSON__True else JSON__False).
 
 Arguments Observe__FromServer {_ _ _}.
 Arguments Observe__FromClient {_ _ _}.
 
-Definition runObserve {T} (oe: observeE Q A S T) : IO T :=
-  match oe in observeE _ _ _ T return _ T with
-  | Observe__FromServer QSync =>
-    command "unison -batch A B";; ret Ayes
-  | Observe__FromServer (QFile r f) =>
+Variant logE : Type -> Set :=
+  Log: string -> logE unit.
+
+Class Is__tE E `{failureE -< E} `{clientE S -< E} `{logE -< E}.
+Notation tE := (failureE +' clientE S +' logE).
+Instance tE_Is__tE: Is__tE tE. Defined.
+
+Definition toClient T (oe: oE _ _ _ T) : itree tE T :=
+  match oe with
+  | (oe|) =>
+    match oe in observeE _ _ _ T return _ T with
+    | Observe__FromServer q =>
+      j <- embed Client__Exec (JEncode__Q q);;
+      match JDecode__A j with
+      | inl str =>
+        embed Log str;;
+        throw ("Cannot parse response IR: " ++ Printer.to_string j)
+      | inr a => ret a
+      end
+    | Observe__FromClient s =>
+      j <- embed Client__Gen s;;
+      match JDecode__Q j with
+      | inl str =>
+        embed Log str;;
+        throw ("Cannot parse request IR: " ++ Printer.to_string j)
+      | inr q => ret q
+      end
+    end
+  | (|Throw str) => throw str
+  end.
+
+Module FileTypes: AsyncTestSIG.
+
+Definition gen_state := S.
+Definition otherE := logE.
+Definition other_handler {T} (oe: otherE T) : IO T :=
+  let 'Log str := oe in
+  prerr_endline str.
+
+Open Scope list_scope.
+
+Definition exec_request (j: IR) : IO IR :=
+  match JDecode__Q j with
+  | inl str => failwith str
+  | inr QSync =>
+    command "unison -batch A B";; ret JSON__True
+  | inr (QFile r f) =>
     let base: path := if r is R1 then ["A"] else ["B"] in
-    tee $
     match f with
-    | Fls    p   => Als ∘ map obasename <$> ols (flatten (base ++ p))
+    | Fls    p   => JEncode__list ∘ map obasename <$> ols (flatten (base ++ p))
     | Fread  p   => read_file (base ++ p)
     | Fwrite p s => write_file (base ++ p) s
-    | Fmkdir p   => b <- omkdir (flatten (base ++ p));;
-                   ret (if b : bool then Ayes else Ano)
-    | Frm    p   => b <- orm [flatten (base ++ p)];;
-                   ret (if b : bool then Ayes else Ayes )
+    | Fmkdir p   => JEncode__bool <$> omkdir (flatten (base ++ p))
+    | Frm    p   => JEncode__bool <$> orm [flatten (base ++ p)]
     end
-  | Observe__FromClient s =>
-    tee $
-    let '(g, a, b) := s in
-    r <- io_choose [R1; R2];;
-    p <- gen_many 3 gen_string;;
-    c <- gen_string;;
-    io_choose [QSync;
-              QFile r (Fls p);
-              QFile r (Fread p);
-              QFile r (Fwrite p c);
-              QFile r (Fmkdir p);
-              QFile r (Frm p)]
   end.
 
-Definition runO T (oe: oE Q A S T) : IO T :=
-  match oe with
-  | (oe|)        => runObserve oe
-  | (|Throw str) => failwith str
-  end.
+Open Scope jexp_scope.
 
+Definition gen_step (s: gen_state) (t: traceT) : IO jexp :=
+  let '(g, a, b) := s in
+  target <- io_choose [1; 2];;
+  method <- io_choose ["ls"; "read"; "mkdir"; "write"];;
+  (* Todo: choose path from ls response. *)
+  p <- io_choose (pathsOf g ++ pathsOf a ++ pathsOf b);;
+  c <- gen_string;;
+  io_choose [Jexp__Const JSON__Null;
+            (jobj "target" target +
+             jobj "method" method +
+             jobj "path"    p     +
+             jobj "content" c)].
+
+Close Scope jexp_scope.
+
+Definition tester_state := unit.
+Definition tester_init: IO tester_state :=
+  orm ["A"; "B"];;
+  omkdir "A";;
+  omkdir "B";;
+  command "unison -batch A B";;
+  ret tt.
 Definition fileServer   := serverOf qstep initS.
 Definition fileObserver := observe fileServer.
-Definition fileTester   :=
-  orm ["A"; "B"];; omkdir "A";; omkdir "B";; command "unison -batch A B";;
-  interp_io runO fileObserver.
+
+Definition tester (_: tester_state) := interp toClient fileObserver.
+
+End FileTypes.
+
+Module FileTest := AsyncTest FileTypes.
+
+Definition fileTester: IO unit :=
+  b <- FileTest.test;;
+  prerr_endline (if b : bool then "Passed" else "Failed").
