theories/Syntax.v
@@ -1,3 +1,7 @@
+From JSON Require Import
+     Encode
+     Decode
+     Operator.
 From FileSync Require Export
      File.
 From ExtLib Require Export
@@ -7,6 +11,8 @@ From ExtLib Require Export
      RelDec.
 From Ceres Require Export
      Ceres.
+Import
+  JNotations.
 
 Variant F :=
   Fls    (p: path)
@@ -61,10 +67,63 @@ Instance Serialize__F: Serialize F :=
          end.
 
 Instance Serialize__R: Serialize R :=
-  fun r => Atom (if r is R1 then "R1" else "R2").
+  fun r => Atom (if r is R1 then 1 else 2)%Z.
 
 Instance Serialize__Q: Serialize Q :=
   fun q => if q is QFile r f then [to_sexp r; to_sexp f]
          else Atom "Sync".
 
 Close Scope sexp_scope.
+
+Instance JDecode__A: JDecode A :=
+  fun j =>
+    (b <- JDecode__bool j;; inr (if b : bool then Ayes else Ano))
+      <|> Aread <$> JDecode__string j
+      <|> Als   <$> decode__list    j.
+
+Close Scope list_scope.
+
+Instance JDecode__R: JDecode R :=
+  fun j =>
+    r <- JDecode__nat j;;
+    match r with
+    | 1 => inr R1
+    | 2 => inr R2
+    | _ => inl $ "Invalid replica: " ++ to_string r
+    end.
+
+Instance JDecode__path: JDecode path :=
+  @decode__list string _.
+
+Instance JDecode__Q: JDecode Q :=
+  fun j =>
+    (r <- dpath "target" j;;
+     m <- dpath "method" j;;
+     p <- dpath "path"   j;;
+     f <- (match m with
+           | "ls"    => inr $ Fls p
+           | "read"  => inr $ Fread p
+           | "mkdir" => inr $ Fmkdir p
+           | "write" => Fwrite p <$> dpath "content" j
+           | _ => inl $ "Invalid method: " ++ m
+           end);;
+    inr (QFile r f))%string
+    <|> (JDecode__unit j;; inr QSync).
+
+Instance JEncode__F: JEncode F :=
+  fun f =>
+    match f with
+    | Fls    p   => jobj "method" "ls"    + jobj "path" p
+    | Frm    p   => jobj "method" "rm"    + jobj "path" p
+    | Fread  p   => jobj "method" "read"  + jobj "path" p
+    | Fmkdir p   => jobj "method" "mkdir" + jobj "path" p
+    | Fwrite p c => jobj "method" "write" + jobj "path" p + jobj "content" c
+    end.
+
+Instance JEncode__Q: JEncode Q :=
+  fun q =>
+    match q with
+    | QSync => JSON__Null
+    | QFile r f =>
+      jobj "target" (if r is R1 then 1 else 2) + JEncode__F f
+    end.
